ProvingItemIndex.fst
@@ -1,0 +1,410 @@
+module ProvingItemIndex
+
+open FStar.Classical 
+open FStar.IO
+open FStar.Printf
+open FStar.List
+open FStar.List.Tot.Base
+
+type english_letters =
+  | A
+  | B
+  | C 
+  | D
+  | E
+  | F 
+  | G
+  | H
+  | I 
+  | J
+  | K
+  | L 
+  | M 
+  | N 
+  | O 
+  | P 
+  | Q 
+  | R 
+  | S 
+  | T 
+  | U 
+  | V 
+  | W 
+  | X 
+  | Y 
+  | Z
+
+val alphabet : list english_letters 
+let alphabet = [A;B;C;D;E;F;G;H;I;J;K;M;N;O;P;Q;R;S;T;U;V;W;X;Y;Z]
+  
+val text : list english_letters
+let text = [E;A;A;A;X;A;B;X;A;A;X;B;A;X;B;A;A;A;B;A;B;B]
+
+val pattern : list english_letters
+let pattern = [E;A;A;A;X;E;C;F;C]
+
+val alphabet_length : (i:nat{i > 0})
+let alphabet_length = length alphabet
+
+let rec create_bc (i:nat) : Tot (list int) (decreases i) 
+  =match i with
+      | 0 -> []
+      | _ -> (-1) :: (create_bc (i-1))
+
+let rec length_create_bc_is_positive (i:nat)
+  : Lemma (ensures length (create_bc i) >= 0)
+  = match i with
+    | 0 -> ()
+    | _ -> length_create_bc_is_positive (i - 1)
+
+let rec length_create_bc_is_i (i:nat) :
+   Lemma (ensures (length (create_bc i) = i)) =
+   match i with 
+     | 0 -> ()
+     | _ -> length_create_bc_is_i (i - 1)
+
+let rec index_n_bc_is_minusone (i:nat) :
+  Lemma (ensures 
+        (let l = (create_bc i) in 
+         forall (n:nat). n < length l ==> index l n = -1))
+  = match i with
+    | 0 -> ()
+    | _ -> index_n_bc_is_minusone (i - 1)
+
+let bc : list int = create_bc alphabet_length
+
+let bc_length_is_positive = length_create_bc_is_positive alphabet_length
+let bc_length_is_alphabet = length_create_bc_is_i alphabet_length
+let bc_nth_element_is_minusone = index_n_bc_is_minusone alphabet_length
+
+//indices
+val item_index (#a:eqtype) (item:a) (l:list a) (i:nat) : list nat
+let rec item_index item l i
+  = match l with 
+    | [] -> []
+    | hd :: tl -> if hd = item
+                  then i :: item_index item tl (i + 1)
+                  else item_index item tl (i + 1)
+
+let rec item_indices_is_in_interval (#a:eqtype) (item:a) (l:list a) (i:nat) (x:nat)
+  : Lemma (ensures mem x (item_index item l i) ==> i <= x)
+  = match l with 
+    | [] -> () 
+    | hd :: tl -> item_indices_is_in_interval item tl (i + 1) x 
+
+let rec index_increases_with_one_when_element_is_added (#a:eqtype) (item:a) (l:list a) (i:nat{i > 0}) (el:a)
+  : Lemma (ensures mem (i - 1) (item_index item l 0) = false ==> mem i (item_index item (el :: l) 0) = false)
+  = match l with 
+    | [] -> ()
+    | hd :: tl -> match i with 
+                  | 1 -> if hd = item 
+                         then ()
+                         else (
+                          if el = item 
+                          then (
+                           
+                          )
+                         )
+                  | _ -> admit()
+
+let lemma_aux3 (#a:eqtype) (item:a) (tl:list a) (i:nat{i > 0})
+  : Lemma (ensures mem (i - 1) (item_index item tl 0) = false ==> mem i (0 :: item_index item tl 1) = false)
+  = admit()
+
+let item_list_length_is_zero_if_the_list_length_is_zero (#a:eqtype) (l:list a)
+  : Lemma (requires l = [])
+          (ensures forall (item:a). length (item_index item l 0) = 0)
+  = ()
+
+let item_head (#a:eqtype) (l:list a)
+  : Lemma (requires length l >= 1)
+          (ensures forall (item:a). length (item_index item [hd l] 0) <= 1)
+  = ()
+
+let rec item_head_not_equal (#a:eqtype) (l:list a)
+  : Lemma (requires length l >= 1)
+          (ensures forall (item:a). hd l <> item ==> length (item_index item [hd l] 0) = 0)
+  = match l with
+    | last -> ()
+    | hd :: tl -> item_head_not_equal tl
+
+let rec item_head_equal (#a:eqtype) (l:list a)
+  : Lemma (requires length l >= 1)
+          (ensures forall (item:a). hd l = item ==> length (item_index item [hd l] 0) = 1)
+  = match l with
+    | last -> ()
+    | hd :: tl -> item_head_equal tl
+
+let rec item_head_count (#a:eqtype) (l:list a)
+  : Lemma (requires length l >= 1) 
+          (ensures forall (item:a). length (item_index item [hd l] 0) = count item [hd l])
+  = match l with 
+    | last -> ()
+    | hd :: tl -> item_head_count tl
+
+let item_empty_list_count (a:eqtype)
+  : Lemma (ensures forall (item:a). length (item_index item [] 0) = count item [])
+  = ()
+
+let rec item_tail_count (#a:eqtype) (l:list a)
+  : Lemma (requires length l >= 1) 
+          (ensures forall (item:a). length (item_index item (tl l) 0) = count item (tl l))
+  = match l with 
+    | last -> admit()
+    | hd :: tl -> admit(item_tail_count tl)
+
+let rec item_tail (#a:eqtype) (l:list a)
+  : Lemma (requires length l >= 1)
+          (ensures forall (item:a). length (item_index item l 0) = length (item_index item [hd l] 0) + length (item_index item (tl l) 1))
+  = match l with 
+    | final -> ()
+    | hd :: tl -> item_tail tl
+
+let rec count_tail (#a:eqtype) (l:list a)
+  : Lemma (requires length l >= 1)
+          (ensures forall (item:a). count item l = count item [hd l] + count item (tl l))
+  = match l with
+    | final -> ()
+    | hd :: tl -> count_tail tl
+
+let rec item_list_has_correct_length (#a:eqtype) (l:list a) (i:nat)
+  : Lemma (ensures forall (item:a). length (item_index item l i) = count item l)
+  = match l with 
+    | [] -> ()
+    | hd :: tl -> item_list_has_correct_length tl (i + 1)
+
+let rec item_index_is_empty (#a:eqtype) (l:list a)
+  : Lemma (ensures forall (item:a). (l = []) \/ (forall (i:nat{i < length l}). index l i <> item) ==> item_index item l 0 = [])
+  = match l with
+    | [] -> ()
+    | hd :: tl -> admit(item_index_is_empty tl)
+
+let rec reunite_the_list (#a:eqtype) (l:list a)
+  : Lemma (requires length l >= 1)
+          (ensures l = append [hd l] (tl l))
+  = match l with 
+    | final -> ()
+    | hd :: tl -> reunite_the_list tl
+
+let rec item_tail_not_equal (#a:eqtype) (l:list a)
+  : Lemma (requires length l >= 1)
+          (ensures forall (item:a). item_index item l 0 = append (item_index item [hd l] 0) (item_index item (tl l) 1))
+  = match l with
+    | final -> ()
+    | hd :: tl -> item_tail_not_equal tl
+
+let rec item_list_has_length_at_least_zero (#a:eqtype) (l:list a) 
+  : Lemma (ensures forall (item:a). length (item_index item l 0) >= 0)
+  = match l with
+    | [] -> ()
+    | hd :: tl -> item_list_has_length_at_least_zero tl
+
+let rec item_has_at_most_length_l_occurrences (#a:eqtype) (l:list a)
+  : Lemma (ensures forall (item:a). count item l <= length l)
+  = match l with 
+    | [] -> ()
+    | hd :: tl -> item_has_at_most_length_l_occurrences tl
+
+//correct store of indexes
+
+let rec exists_item_zero_then_correct_index (#a:eqtype) (l:list a)
+  : Lemma (requires length l > 0)
+          (ensures forall (item:a).  index l 0 = item ==> mem 0 (item_index item l 0))
+  = match l with
+    | [last] -> ()
+    | hd :: tl -> exists_item_zero_then_correct_index tl
+
+let rec exists_item_one_then_correct_index (#a:eqtype) (l:list a)
+  : Lemma (requires length l > 1)
+          (ensures forall (item:a).  index l 1 = item ==> mem 1 (item_index item l 0))
+  = match length l with
+    | 2 -> ()
+    | _ -> exists_item_one_then_correct_index (tl l)
+
+let rec exists_item_i_then_correct_index (#a:eqtype) (l:list a) (i:nat)
+  : Lemma (requires length l > i)
+          (ensures forall (item:a). index l i = item ==> mem i (item_index item l 0))
+  = let j = i + 1 in
+    match length l with
+    | j -> admit()
+    | _ -> exists_item_i_then_correct_index (tl l) i
+
+let rec index_is_or_is_not_item_is_or_is_not_mem (#a:eqtype) (l:list a)
+  : Lemma (ensures forall (item:a). forall (i:nat{i < length l}). (index l i = item || index l i <> item) ==> (mem i (item_index item l 0) = true || mem i (item_index item l 0) = false))
+  = match l with
+    | [] -> ()
+    | hd :: tl -> index_is_or_is_not_item_is_or_is_not_mem tl
+
+let rec index_is_not_item_is_not_mem_aux (#a:eqtype) (l:list a) (item:a) (i:nat{i < length l})
+  : Lemma (ensures index l i <> item ==> mem i (item_index item l 0) = false)
+  = match l with
+    | [] -> ()
+    | hd :: tl -> match i with 
+                  | 0 -> if hd = item 
+                         then ()
+                         else (
+                          //assert(item <> hd);
+                          //assert(index l i = hd);
+                          //assert(index l i <> item);
+                          //assert(item_index item l 0 = item_index item tl (i + 1));
+                          item_indices_is_in_interval item tl (i + 1) i
+                         )
+                  | _ -> //assert(index l i = index tl (i - 1));
+                         if hd = item 
+                         then 
+                         //assert(mem i (item_index item l 0) = mem i (0 :: item_index item tl 1));
+                         lemma_aux3 item tl i
+                         else 
+                         //assert(mem i (item_index item l 0) = mem i (item_index item tl 1));
+                         lemma_aux2 item tl i hd;
+                         index_is_not_item_is_not_mem_aux tl item (i - 1)
+
+let rec index_is_not_item_is_not_mem (#a:eqtype) (l:list a)
+  : Lemma (ensures forall (item:a). forall (i:nat{i < length l}). index l i <> item ==> mem i (item_index item l 0) = false)
+  = match l with
+    | [] -> ()
+    | hd :: tl -> admit(index_is_not_item_is_not_mem tl)
+
+let rec exists_item_then_correct_index (#a:eqtype) (l:list a)
+  : Lemma (ensures forall (item:a). forall (i:nat{i < length l}). index l i = item ==> mem i (item_index item l 0))
+  = match l with
+    | [] -> ()
+    | hd :: tl -> admit(exists_item_then_correct_index tl)
+
+let rec correct_index_then_exists_item (#a:eqtype) (l:list a)
+  : Lemma (ensures forall (item:a). forall (n:nat{n < length l}). mem n (item_index item l 0) ==> index l n = item)
+  = match l with
+    | [] -> ()
+    | hd :: tl -> admit(correct_index_then_exists_item tl)
+
+let rec exists_item_index_iff_correct_index (#a:eqtype) (l:list a)
+  : Lemma (ensures forall (item:a). forall (i:nat{i < length l}). index l i = item <==> mem i (item_index item l 0))
+  = match l with
+    | [] -> ()
+    | hd :: tl -> exists_item_index_iff_correct_index tl;
+                  exists_item_then_correct_index l;
+                  correct_index_then_exists_item l
+
+let rec index_is_in_interval (#a:eqtype) (l:list a)
+  : Lemma (ensures forall (item:a). forall (i:nat). mem i (item_index item l 0) = true ==> i >= 0 && i < length l)
+  = match l with 
+    | [] -> ()
+    | hd :: tl -> admit(index_is_in_interval tl)
+
+let rec last_is_in_interval (#a:eqtype) (l:list a)
+  : Lemma (ensures forall (item:a). item_index item l 0 <> [] ==> last (item_index item l 0) >= 0 && last (item_index item l 0) < length l)
+  = match l with
+    | [] -> ()
+    | hd :: tl -> admit(last_is_in_interval tl)
+
+let new_or_old (#a:eqtype) (c:a) (l:list a) : int
+  = if item_index c l 0 <> []
+    then last (item_index c l 0)
+    else -1
+
+let rec not_new_or_old_empty_list (#a:eqtype) (l:list a) 
+  : Lemma (ensures forall (item:a). new_or_old item l = -1 ==> item_index item l 0 = [])
+  = match l with
+    | [] -> ()
+    | hd :: tl -> not_new_or_old_empty_list tl 
+
+let rec empty_list_length_zero (#a:eqtype) (l:list a) 
+  : Lemma (ensures forall (item:a). item_index item l 0 = [] ==> length (item_index item l 0) = 0)
+  = match l with 
+    | [] -> ()
+    | hd :: tl -> empty_list_length_zero tl
+
+let rec length_zero_count_zero (#a:eqtype) (l:list a)
+  : Lemma (ensures forall (item:a). length (item_index item l 0) = 0 ==> count item l = 0)
+  = match l with
+    | [] -> ()
+    | hd :: tl -> length_zero_count_zero tl;
+                  item_list_has_correct_length l 0
+
+let rec count_zero_mem_false (#a:eqtype) (l:list a)
+  : Lemma (ensures forall (item:a). count item l = 0 ==> mem item l = false)
+  = match l with
+    | [] -> ()
+    | hd :: tl -> count_zero_mem_false tl
+                 
+let rec mem_false_not_item (#a:eqtype) (l:list a)
+  : Lemma (ensures forall (item:a). mem item l = false ==> (forall (i:nat). i < length l ==> index l i <> item))
+  = match l with 
+    | [] -> ()
+    | hd :: tl -> mem_false_not_item tl
+
+let rec new_or_old_not_item (#a:eqtype) (l:list a)
+  : Lemma (ensures forall (item:a). new_or_old item l = -1 ==> (forall (i:nat). i < length l ==> index l i <> item))
+  = match l with
+    | [] -> ()
+    | hd :: tl -> new_or_old_not_item tl;
+                  not_new_or_old_empty_list l;
+                  empty_list_length_zero l;
+                  length_zero_count_zero l;
+                  count_zero_mem_false l;
+                  mem_false_not_item l
+
+let rec new_or_old_not_empty_list (#a:eqtype) (l:list a)
+  : Lemma (ensures forall (item:a). new_or_old item l <> -1 ==> item_index item l 0 <> [])
+  = match l with
+    | [] -> ()
+    | hd :: tl -> new_or_old_not_empty_list tl
+
+let rec not_empty_list_length_greater_than_zero (#a:eqtype) (l:list a)
+  : Lemma (ensures forall (item:a). (item_index item l 0 <> [] && last (item_index item l 0) < length l) ==> last (item_index item l 0) >= 0)
+  = match l with
+    | [] -> ()
+    | hd :: tl -> not_empty_list_length_greater_than_zero tl                  
+
+let rec last_list_mem (#a:eqtype) (l:list a)
+  : Lemma (requires length l > 0)
+          (ensures mem (last l) l = true)
+  = match l with
+    | [hd] -> ()
+    | hd :: tl -> last_list_mem tl
+
+let item_index_not_empty (#a:eqtype) (item:a) (l:list a)
+  : Type 
+  = item_index item l 0 <> []
+
+let implication_last_is_in_list (#a:eqtype) (item:a) (l:list a{item_index item l 0 <> []})
+  : Type
+  = last (item_index item l 0) >= 0 ==> mem (last (item_index item l 0)) (item_index item l 0) = true
+
+let length_greater_than_zero_mem (#a:eqtype) (item:a) (l:list a)
+  : Lemma (requires item_index_not_empty item l)
+          (ensures implication_last_is_in_list item l) 
+  = last_list_mem (item_index item l 0)
+
+let length_greater_than_zero_mem_forall (#a:eqtype) (l:list a)
+  : Lemma (ensures forall (item:a). item_index_not_empty ==> implication_last_is_in_list item l)
+  = forall_intro (move_requires (length_greater_than_zero_mem item) l)
+
+let mem_index_is_item (#a:eqtype) (l:list a) (item:a)
+  : Lemma (requires item_index item l 0 <> [] && last (item_index item l 0) < length l)
+          (ensures mem (last (item_index item l 0)) (item_index item l 0) = true ==> index l (last (item_index item l 0)) = item)
+  = exists_item_index_iff_correct_index l;
+    ()
+
+let new_or_old_not_empty_list_correct_item (#a:eqtype) (l:list a) (item:a)
+  : Lemma (requires item_index item l 0 <> [] && last (item_index item l 0) < length l)
+          (ensures new_or_old item l <> -1 ==> index l (last (item_index item l 0)) = item)
+  = new_or_old_not_empty_list l;
+    not_empty_list_length_greater_than_zero l;
+    length_greater_than_zero_mem item l;
+    mem_index_is_item l item;
+    ()
+
+val update_bc (a:list english_letters) : list int
+let rec update_bc a = 
+    match a with 
+        | [] -> []
+        | hd::tl -> (new_or_old hd pattern) :: update_bc tl
+
+let final_bc : list int = update_bc alphabet
+
+let rec final_bc_length_is_alphabet_length (a:list english_letters)
+  : Lemma (ensures length (update_bc a) = length a)
+  = match a with
+      | [] -> ()
+      | hd :: tl -> final_bc_length_is_alphabet_length tl
